code/style-experiments/Hacl.Impl.Curve25519.Generic.fst
@@ -223,15 +223,27 @@ let point_add_and_double_ #s q nq nq_p1 =
    footprint h0 gloc (fun () -> fsub b x2 z2); // b = x2 - z2
    footprint h0 gloc (fun () -> fadd c x3 z3); // c = x3 + z3
    footprint h0 gloc (fun () -> fsub d x3 z3); // d = x3 - z3
+
+   (* CAN RUN IN PARALLEL *)
    footprint h0 gloc (fun () -> fmul d d a);   // d = da = d * a 
    footprint h0 gloc (fun () -> fmul c c b);   // c = cb = c * b
+//   footprint h0 gloc (fun () -> fmul2 d c d a c b);   // c = cb = c * b
+   
    footprint h0 gloc (fun () -> fadd x3 d c);  // x3 = da + cb
-   footprint h0 gloc (fun () -> fsqr x3 x3);   // x3 = (da + cb) ^ 2
    footprint h0 gloc (fun () -> fsub z3 d c);  // z3 = da - cb
+
+   (* CAN RUN IN PARALLEL *)
+   footprint h0 gloc (fun () -> fsqr x3 x3);   // x3 = (da + cb) ^ 2
    footprint h0 gloc (fun () -> fsqr z3 z3);   // z3 = (da - cb) ^ 2
+//   footprint h0 gloc (fun () -> fsqr2 x3 z3 x3 z3);   // z3 = (da - cb) ^ 2
+   
    footprint h0 gloc (fun () -> fmul z3 z3 x1); // z3 = x1 * (da - cb) ^ 2
+
+   (* CAN RUN IN PARALLEL *)
    footprint h0 gloc (fun () -> fsqr c a);     // c = aa = a^2
    footprint h0 gloc (fun () -> fsqr d b);     // d = bb = b^2
+//   footprint h0 gloc (fun () -> fsqr2 c d a b);     // d = bb = b^2
+   
    footprint h0 gloc (fun () -> fmul x2 c d);  // x2 = aa * bb
    footprint h0 gloc (fun () -> fsub b c d);   // b = e = aa - bb
    footprint h0 gloc (fun () -> fmul1 a b (u64 121665)); // a = e * 121665
